src/Helpers/RelationAlgebra.v
@@ -463,14 +463,15 @@ Ltac rel_congruence :=
     solver
   end.
 
+(* TODO: maintain a fast version of this tactic *)
 Ltac norm :=
-  rewrite ?bind_assoc, ?bind_left_id in *;
+  rewrite ?bind_assoc, ?bind_left_id, ?bind_star_unit in *;
   repeat (setoid_rewrite bind_assoc ||
           setoid_rewrite bind_left_id ||
-          setoid_rewrite rel_or_assoc);
+          setoid_rewrite rel_or_assoc ||
+          setoid_rewrite bind_star_unit);
   repeat match goal with
          | [ H: _ |- _ ] => setoid_rewrite bind_assoc in H
          | [ H: _ |- _ ] => setoid_rewrite bind_left_id in H
-         | [ H: _ |- _ ] => setoid_rewrite rel_or_assoc in H
          end;
   try reflexivity.
