src/Spec/Layer.v
@@ -38,9 +38,9 @@ Section Layers.
   Notation compile_op := impl.(compile_op).
   Notation recover := impl.(recover).
 
-  Definition compile_op_refines_step (abs: AState -> CState -> Prop) :=
+  Definition compile_op_refines_step (absr: relation AState CState unit) :=
     forall T (op: Op T),
-      crash_refines abs c_sem
+      crash_refines absr c_sem
                     (compile_op op) recover
                     (a_sem.(step) op)
                     (* same as [(pure tt + (a_sem.(step) op;; pure tt));;
@@ -49,8 +49,8 @@ Section Layers.
                     (a_sem.(crash_step) +
                      (a_sem.(step) op;; a_sem.(crash_step))).
 
-  Definition recovery_refines_noop (abs: AState -> CState -> Prop) :=
-    crash_refines abs c_sem
+  Definition recovery_refines_noop (absr: relation AState CState unit) :=
+    crash_refines absr c_sem
                   recover
                   recover
                   any (* normal behavior of recovery is irrelevant, we never ask
@@ -58,9 +58,9 @@ Section Layers.
                   (a_sem.(crash_step)).
 
   Record LayerRefinement :=
-    { abs: AState -> CState -> Prop;
-      compile_op_ok : compile_op_refines_step abs;
-      recovery_ok : recovery_refines_noop abs;
+    { absr: relation AState CState unit;
+      compile_op_ok : compile_op_refines_step absr;
+      recovery_ok : recovery_refines_noop absr;
       (* TODO: init_ok *) }.
 
   Fixpoint compile T (p: a_proc T) : c_proc T :=
@@ -77,7 +77,7 @@ Section Layers.
   Opaque exec_recover.
 
   Theorem compile_ok : forall T (p: a_proc T) R (rec: a_proc R),
-      crash_refines rf.(abs) c_sem
+      crash_refines rf.(absr) c_sem
                     (compile p) (Bind recover (fun _ => compile rec))
                     (a_sem.(exec) p)
                     (a_sem.(rexec) p rec).
@@ -95,9 +95,28 @@ Section Layers.
       setoid_rewrite <- bind_assoc at 2.
       setoid_rewrite <- bind_assoc at 1.
       rewrite H0; norm.
-      setoid_rewrite bind_star_unit.
       rewrite ?bind_dist_r; norm.
       apply rel_or_elim.
+      + rewrite <- exec_crash_noop; norm.
+        rel_congruence.
+        admit.
+      + unfold exec_crash.
+        rewrite <- rel_or_intror; norm.
+        rel_congruence.
+        rel_congruence.
+        admit.
+    - let H := fresh "Hnoop" in
+      pose proof (rf.(recovery_ok)) as H;
+        unfold recovery_refines_noop, crash_refines in H;
+        propositional.
+      split; simpl.
+      + unfold refines; norm.
+      + unfold refines in *; norm.
+        rewrite <- exec_crash_noop; norm.
+        (* TODO: repeating a proof above about c_exec_recover of [recover;
+        compile rec] *)
+        setoid_rewrite exec_recover_bind.
+        unfold rexec in H0.
   Abort.
 
 End Layers.
